simplify proof of finv

code/curve25519/Hacl.Impl.Curve25519.Finv.fst
@@ -6,25 +6,25 @@ open FStar.Mul
 
 open Lib.IntTypes
 open Lib.Buffer
-open Lib.ByteBuffer
 
 open Hacl.Impl.Curve25519.Fields
 
 module ST = FStar.HyperStack.ST
-
 module C = Hacl.Impl.Curve25519.Fields.Core
-
 module S = Hacl.Spec.Curve25519.Finv
 module P = Spec.Curve25519
 
-#reset-options "--z3rlimit 50 --fuel 0 --ifuel 1 --using_facts_from '* -FStar.Seq' --record_options"
+#reset-options "--z3rlimit 50 --fuel 0 --ifuel 0"
+
 
 noextract
 val fsquare_times_inv: #s:field_spec -> h:mem -> f:felem s -> Type0
 let fsquare_times_inv #s h f =
+  allow_inversion field_spec;
   match s with
   | M51 -> C.f51_felem_fits h f (1, 2, 1, 1, 1)
   | M64 -> True
+
 
 val fsqr_s:
     #s:field_spec
@@ -46,12 +46,15 @@ val fsqr_s:
 let fsqr_s #s out f1 tmp =
   C.fsqr #s out f1 tmp
 
+
 noextract
 val fmuls_pre: #s:field_spec -> h:mem -> f1:felem s -> f2:felem s -> Type0
 let fmuls_pre #s h f1 f2 =
+  allow_inversion field_spec;
   match s with
   | M51 -> f51_felem_fits h f1 (1, 2, 1, 1, 1) /\ f51_felem_fits h f2 (1, 2, 1, 1, 1)
   | M64 -> True
+
 
 val fmul_s:
     #s:field_spec
@@ -76,7 +79,7 @@ val fmul_s:
 let fmul_s #s out f1 f2 tmp =
   C.fmul #s out f1 f2 tmp
 
-#set-options "--fuel 1 --ifuel 1"
+
 val fsquare_times:
     #s:field_spec
   -> o:felem s
@@ -93,32 +96,165 @@ val fsquare_times:
     (ensures  fun h0 _ h1 ->
       modifies (loc o |+| loc tmp) h0 h1 /\
       fsquare_times_inv h1 o /\
-      feval h1 o == S.pow (feval #s h0 i) (pow2 (v n)))
+      feval h1 o == S.fsquare_times (feval #s h0 i) (v n))
 [@ Meta.Attribute.specialize ]
 let fsquare_times #s o inp tmp n =
   let h0 = ST.get() in
   fsqr_s #s o inp tmp;
-  let h1 = ST.get() in
   S.lemma_pow_one (feval h0 inp);
   S.lemma_pow_add (feval h0 inp) 1 1;
   assert_norm (pow2 1 = 2);
+
   let inv (h:mem) (i:nat{i < v n}) =
-    modifies (loc o |+| loc tmp) h0 h /\ fsquare_times_inv #s h o /\
+    modifies (loc o |+| loc tmp) h0 h /\
+    fsquare_times_inv #s h o /\
     feval h o == S.pow (feval #s h0 inp) (pow2 (i + 1)) in
+
+  let h1 = ST.get () in
+  assert (inv h1 0);
+
   Lib.Loops.for 0ul (n -! 1ul) inv
   (fun i ->
     let h2 = ST.get () in
     fsqr_s #s o o tmp;
-    let h3 = ST.get () in
     S.lemma_pow_one (feval h2 o);
     S.lemma_pow_add (feval h2 o) 1 1;
     S.lemma_pow_mul (feval #s h0 inp) (pow2 (v i + 1)) (pow2 1);
-    assert_norm (pow2 (v i + 1) * pow2 1 = pow2 (v i + 2)))
+    Math.Lemmas.pow2_plus (v i + 1) 1;
+    assert (pow2 (v i + 1) * pow2 1 = pow2 (v i + 2)))
 
-#set-options "--z3rlimit 300 --fuel 0 --ifuel 1"
+
+val finv1:
+    #s:field_spec{range (4 * v (nlimb s)) U32}
+  -> i:felem s
+  -> t1:lbuffer (limb s) (4ul *! nlimb s)
+  -> tmp:felem_wide2 s ->
+  Stack unit
+  (requires fun h0 ->
+    live h0 i /\ live h0 t1 /\ live h0 tmp /\
+    disjoint i t1 /\ disjoint i tmp /\ disjoint t1 tmp /\
+    fsquare_times_inv h0 i)
+  (ensures  fun h0 _ h1 ->
+    modifies (loc t1 |+| loc tmp) h0 h1 /\
+   (let as : felem s = gsub t1 0ul (nlimb s) in
+    let bs : felem s = gsub t1 (nlimb s) (nlimb s) in
+    let a = S.fsquare_times (feval h0 i) 1 in
+    let t0 = S.fsquare_times a 2 in
+    let b = P.fmul t0 (feval h0 i) in
+    let a = P.fmul b a in
+    let t0 = S.fsquare_times a 1 in
+    let b = P.fmul t0 b in
+    let t0 = S.fsquare_times b 5 in
+    let b = P.fmul t0 b in
+    feval h1 as == a /\ fsquare_times_inv h1 as /\
+    feval h1 bs == b /\ fsquare_times_inv h1 bs))
+
+[@ Meta.Attribute.inline_ ]
+let finv1 #s i t1 tmp =
+  let h0 = ST.get () in
+  let a : felem s = sub t1 0ul (nlimb s) in
+  let b : felem s = sub t1 (nlimb s) (nlimb s) in
+  let c : felem s = sub t1 (2ul *! nlimb s) (nlimb s) in
+  let t0 : felem s = sub t1 (3ul *! nlimb s) (nlimb s) in
+  let tmp1 : felem_wide s = sub tmp 0ul (nwide s) in
+  (* 2 *) fsquare_times #s a i tmp1 1ul;
+  (* 8 *) fsquare_times #s t0 a tmp1 2ul;
+  (* 9 *) fmul_s #s b t0 i tmp;
+  (* 11 *) fmul_s #s a b a tmp;
+  (* 22 *) fsquare_times #s t0 a tmp1 1ul;
+  (* 2^5 - 2^0 = 31 *) fmul_s #s b t0 b tmp;
+  (* 2^10 - 2^5 *) fsquare_times #s t0 b tmp1 5ul;
+  (* 2^10 - 2^0 *) fmul_s #s b t0 b tmp
+
+
+val finv2:
+    #s:field_spec{range (4 * v (nlimb s)) U32}
+  -> t1:lbuffer (limb s) (4ul *! nlimb s)
+  -> tmp:felem_wide2 s ->
+  Stack unit
+  (requires fun h0 ->
+    live h0 t1 /\ live h0 tmp /\ disjoint t1 tmp /\
+   (let as : felem s = gsub t1 0ul (nlimb s) in
+    let bs : felem s = gsub t1 (nlimb s) (nlimb s) in
+    fsquare_times_inv h0 as /\ fsquare_times_inv h0 bs))
+  (ensures  fun h0 _ h1 ->
+    modifies (loc t1 |+| loc tmp) h0 h1 /\
+   (let as : felem s = gsub t1 0ul (nlimb s) in
+    let bs : felem s = gsub t1 (nlimb s) (nlimb s) in
+    let cs : felem s = gsub t1 (2ul *! nlimb s) (nlimb s) in
+    let t0 = S.fsquare_times (feval h0 bs) 10 in
+    let c = P.fmul t0 (feval h0 bs) in
+    let t0 = S.fsquare_times c 20 in
+    let t0 = P.fmul t0 c in
+    let t0 = S.fsquare_times t0 10 in
+    let b = P.fmul t0 (feval h0 bs) in
+    let t0 = S.fsquare_times b 50 in
+    let c = P.fmul t0 b in
+    feval h1 as == feval h0 as /\ fsquare_times_inv h1 as /\
+    feval h1 bs == b /\ fsquare_times_inv h1 bs /\
+    feval h1 cs == c /\ fsquare_times_inv h1 cs))
+
+[@ Meta.Attribute.inline_ ]
+let finv2 #s t1 tmp =
+  let h0 = ST.get () in
+  let a : felem s = sub t1 0ul (nlimb s) in
+  let b : felem s = sub t1 (nlimb s) (nlimb s) in
+  let c : felem s = sub t1 (2ul *! nlimb s) (nlimb s) in
+  let t0 : felem s = sub t1 (3ul *! nlimb s) (nlimb s) in
+  let tmp1 : felem_wide s = sub tmp 0ul (nwide s) in
+  (* 2^20 - 2^10 *) fsquare_times #s t0 b tmp1 10ul;
+  (* 2^20 - 2^0 *) fmul_s #s c t0 b tmp;
+  (* 2^40 - 2^20 *) fsquare_times #s t0 c tmp1 20ul;
+  (* 2^40 - 2^0 *) fmul_s #s t0 t0 c tmp;
+  (* 2^50 - 2^10 *) fsquare_times #s t0 t0 tmp1 10ul;
+  (* 2^50 - 2^0 *) fmul_s #s b t0 b tmp;
+  (* 2^100 - 2^50 *) fsquare_times #s t0 b tmp1 50ul;
+  (* 2^100 - 2^0 *) fmul_s #s c t0 b tmp
+
+
+val finv3:
+    #s:field_spec{range (4 * v (nlimb s)) U32}
+  -> t1:lbuffer (limb s) (4ul *! nlimb s)
+  -> tmp:felem_wide2 s ->
+  Stack unit
+  (requires fun h0 ->
+    live h0 t1 /\ live h0 tmp /\ disjoint t1 tmp /\
+   (let as : felem s = gsub t1 0ul (nlimb s) in
+    let bs : felem s = gsub t1 (nlimb s) (nlimb s) in
+    let cs : felem s = gsub t1 (2ul *! nlimb s) (nlimb s) in
+    fsquare_times_inv h0 as /\ fsquare_times_inv h0 bs /\
+    fsquare_times_inv h0 cs))
+  (ensures  fun h0 _ h1 ->
+    modifies (loc t1 |+| loc tmp) h0 h1 /\
+   (let as : felem s = gsub t1 0ul (nlimb s) in
+    let bs : felem s = gsub t1 (nlimb s) (nlimb s) in
+    let cs : felem s = gsub t1 (2ul *! nlimb s) (nlimb s) in
+    let ts0 : felem s = gsub t1 (3ul *! nlimb s) (nlimb s) in
+    let t0 = S.fsquare_times (feval h0 cs) 100 in
+    let t0 = P.fmul t0 (feval h0 cs) in
+    let t0 = S.fsquare_times t0 50 in
+    let t0 = P.fmul t0 (feval h0 bs) in
+    let t0 = S.fsquare_times t0 5 in
+    feval h1 as == feval h0 as /\ fsquare_times_inv h1 as /\
+    feval h1 ts0 == t0 /\ fsquare_times_inv h1 ts0))
+
+[@ Meta.Attribute.inline_ ]
+let finv3 #s t1 tmp =
+  let h0 = ST.get () in
+  let a : felem s = sub t1 0ul (nlimb s) in
+  let b : felem s = sub t1 (nlimb s) (nlimb s) in
+  let c : felem s = sub t1 (2ul *! nlimb s) (nlimb s) in
+  let t0 : felem s = sub t1 (3ul *! nlimb s) (nlimb s) in
+  let tmp1 : felem_wide s = sub tmp 0ul (nwide s) in
+  (* 2^200 - 2^100 *) fsquare_times #s t0 c tmp1 100ul;
+  (* 2^200 - 2^0 *) fmul_s #s t0 t0 c tmp;
+  (* 2^250 - 2^50 *) fsquare_times #s t0 t0 tmp1 50ul;
+  (* 2^250 - 2^0 *) fmul_s #s t0 t0 b tmp;
+  (* 2^255 - 2^5 *) fsquare_times #s t0 t0 tmp1 5ul
+
 
 val finv0:
-    #s:field_spec
+    #s:field_spec{range (4 * v (nlimb s)) U32}
   -> i:felem s
   -> t1:lbuffer (limb s) (4ul *! nlimb s)
   -> tmp:felem_wide2 s
@@ -135,6 +271,7 @@ val finv0:
       fsquare_times_inv h1 a /\
       fsquare_times_inv h1 t0 /\
       (feval h1 a, feval h1 t0) == (a_s, t0_s)))
+
 [@ Meta.Attribute.inline_ ]
 let finv0 #s i t1 tmp =
   let h0 = ST.get () in
@@ -142,37 +279,15 @@ let finv0 #s i t1 tmp =
   let b : felem s = sub t1 (nlimb s) (nlimb s) in
   let c : felem s = sub t1 (2ul *! nlimb s) (nlimb s) in
   let t0 : felem s = sub t1 (3ul *! nlimb s) (nlimb s) in
-  let tmp1 : felem_wide s = sub tmp 0ul (nwide s) in
-  (* 2 *) fsquare_times #s a i tmp1 1ul;
-  (* 8 *) fsquare_times #s t0 a tmp1 2ul;
-  (* 9 *) fmul_s #s b t0 i tmp;
-  (* 11 *) fmul_s #s a b a tmp;
-  (* 22 *) fsquare_times #s t0 a tmp1 1ul;
-  (* 2^5 - 2^0 = 31 *) fmul_s #s b t0 b tmp;
-  (* 2^10 - 2^5 *) fsquare_times #s t0 b tmp1 5ul;
-  (* 2^10 - 2^0 *) fmul_s #s b t0 b tmp;
-  (* 2^20 - 2^10 *) fsquare_times #s t0 b tmp1 10ul;
-  (* 2^20 - 2^0 *) fmul_s #s c t0 b tmp;
-  (* 2^40 - 2^20 *) fsquare_times #s t0 c tmp1 20ul;
-  (* 2^40 - 2^0 *) fmul_s #s t0 t0 c tmp;
-  (* 2^50 - 2^10 *) fsquare_times #s t0 t0 tmp1 10ul;
-  (* 2^50 - 2^0 *) fmul_s #s b t0 b tmp;
-  (* 2^100 - 2^50 *) fsquare_times #s t0 b tmp1 50ul;
-  (* 2^100 - 2^0 *) fmul_s #s c t0 b tmp;
-  (* 2^200 - 2^100 *) fsquare_times #s t0 c tmp1 100ul;
-  (* 2^200 - 2^0 *) fmul_s #s t0 t0 c tmp;
-  (* 2^250 - 2^50 *) fsquare_times #s t0 t0 tmp1 50ul;
-  let h0' = ST.get () in
-  (* 2^250 - 2^0 *) fmul_s #s t0 t0 b tmp;
-  let h1' = ST.get () in
-  assert (modifies (loc t1 |+| loc tmp) h0' h1');
-  assert (modifies (loc t1 |+| loc tmp) h0 h1');
-  (* 2^255 - 2^5 *) fsquare_times #s t0 t0 tmp1 5ul;
+  finv1 #s i t1 tmp;
+  finv2 #s t1 tmp;
+  finv3 #s t1 tmp;
   let h1 = ST.get () in
   assert (fsquare_times_inv h1 t0);
   assert (fsquare_times_inv h1 a);
   assert (modifies (loc t1 |+| loc tmp) h0 h1);
   assert ( (feval h1 a, feval h1 t0) == S.finv0 (feval h0 i))
+
 
 val finv:
     #s:field_spec
@@ -191,6 +306,7 @@ val finv:
       feval h1 o == P.fpow (feval #s h0 i) (pow2 255 - 21))
 [@ Meta.Attribute.specialize ]
 let finv #s o i tmp =
+  allow_inversion field_spec;
   push_frame();
   let t1 = create (4ul *! nlimb s) (limb_zero s) in
   let h0 = ST.get () in
